Add distinct optimization for algenv

coq/NRAEnv/Optim/TOptimEnv.v
@@ -3083,6 +3083,43 @@ Section TOptimEnv.
                   end) dout); simpl in *; congruence.
   Qed.
 
+  Definition algenv_always_ensures (P:data->Prop) (q:algenv) :=
+      forall
+      (h:list(string*string))
+      (c:list (string*data))
+      (dn_c:Forall (fun d => data_normalized h (snd d)) c)
+      (env:data)
+      (dn_env:data_normalized h env)
+      (x:data)
+      (dn_x:data_normalized h x)
+      (d:data),
+        h ⊢ₑ q @ₑ x ⊣ c;env = Some d -> P d.
+
+  Definition nodupA : algenv -> Prop :=
+    algenv_always_ensures
+      (fun d => match d with
+                | dcoll dl => NoDup dl
+                | _ => True
+                end).
+  
+  Lemma tdup_elim (q:algenv) :
+    nodupA q -> ANUnop ADistinct q  ⇒  q.
+  Proof.
+    red; intros; split; intros; inferer; invcs H3.
+    - trivial.
+    - input_well_typed.
+      dtype_inverter.
+      rewrite rondcoll_dcoll.
+      f_equal.
+      f_equal.
+      apply bindings_type_Forall_normalized in dt_c.
+      apply data_type_normalized in dt_env.
+      apply data_type_normalized in dt_x.
+      specialize (H brand_relation_brands c dt_c env dt_env x dt_x (dcoll dout) eout).
+      simpl in H.
+      apply NoDup_bdistinct; trivial.
+  Qed.
+
 End TOptimEnv.
 
 (* begin hide *)
